src/Employees/Implementation/Employees3.dfy
@@ -84,7 +84,7 @@ method ComputeSolution(input: Input) returns (bs: Solution)
 
   /* Llamada inicial de la vuelta atrás */
   var min := Precalculation(input);
-  EmployeesVA(input, ps, bs, min);
+  //EmployeesVA(input, ps, bs, min);
 
   /* Primera postcondición: bs.Valid(input)
    Se verifica gracias a la postcondición en BT que asegura que bs es válida.
@@ -101,27 +101,27 @@ method ComputeSolution(input: Input) returns (bs: Solution)
   }
 }
 
-method Precalculation(input : Input) returns (min : real)
+method {:only} Precalculation(input : Input) returns (submatrixMin : array<real>)
   requires input.Valid()
-  ensures input.IsMin(min, 0)
+  ensures submatrixMin.Length == input.times.Length0
+  ensures forall i | 0 <= i < input.times.Length0 :: input.IsMin(submatrixMin[i], i)
 {
+  submatrixMin := new real[input.times.Length0];
+  var min := input.times[input.times.Length0 - 1, input.times.Length1 - 1];
+  var i := input.times.Length0 - 1;
+  var j := input.times.Length1 - 1;
 
-  min := input.times[0, 0];
-
-  for i := 0 to input.times.Length0
-    invariant forall f, c | 0 <= f < i && 0 <= c < input.times.Length1 :: min <= input.times[f, c]
-    invariant exists f, c | 0 <= f < input.times.Length0 && 0 <= c < input.times.Length1 :: min == input.times[f,c]
-  {
-    for j := 0 to input.times.Length1
-      invariant forall f, c | 0 <= f < i && 0 <= c < input.times.Length1 :: min <= input.times[f, c]
-      invariant forall c | 0 <= c < j :: min <= input.times[i,c]
-      invariant exists f, c | 0 <= f < input.times.Length0 && 0 <= c < input.times.Length1 :: min == input.times[f, c]
-    {
-      if input.times[i, j] <= min {
-        min := input.times[i, j];
+    while i >= 0 {
+      j := input.times.Length1 - 1;
+      while j >= 0 {
+        if input.times[i, j] <= min {
+          min := input.times[i, j];
+        }
+        j := j - 1;
       }
+      submatrixMin[i] := min;
+      i := i - 1;
     }
-  }
 }
 
 /*
